src/SizeClass.fst
@@ -17,6 +17,7 @@ open Steel.Reference
 module SR = Steel.Reference
 module A = Steel.Array
 
+(*)
 open Utils2
 open SlabsUtils
 
